\documentclass{article}
\begin{document}

\centerline{\sc \large Homework 2}
\vspace{0.5pc}

\centerline{Parth Mehrotra}
\centerline{160005277 - pm619}
\vspace{2pc}


10a.

$$[\lnot p \land (p \lor q)] \rightarrow q$$

\begin{tabular}{c|c|c|c|c|c}
$p$ & $q$ & $\lnot p$ & $p \lor q$ & $\lnot p \land (p \lor q)$  & $\lnot p \land (p \lor q) \rightarrow q$ \\
\hline
0 & 0 & 1	     & 0			& 0							  & 1                                        \\
0 & 1 & 1	     & 1 			& 1							  & 1                                        \\
1 & 0 & 0	     & 1 			& 0							  & 1                                        \\
1 & 1 & 0	     & 1 			& 0							  & 1                                        \\
\end{tabular}


10b.

$$[(p \rightarrow q) \land (q \rightarrow r)] \rightarrow (p \rightarrow r)$$

\begin{tabular}{c|c|c|c|c|c|c|c}
$p$ & $q$ & $r$ & $p \rightarrow q$ & $q \rightarrow r$ & $(p \rightarrow q) \land (q \rightarrow r)$ & $(p \rightarrow r)$ & $[(p \rightarrow q) \land (q \rightarrow r)] \rightarrow (p \rightarrow r)]$ \\
\hline
0 & 0 & 0 & 1 & 1 & 1 & 1 & 1 \\
0 & 0 & 1 & 1 & 1 & 1 & 1 & 1 \\
0 & 1 & 0 & 1 & 0 & 0 & 1 & 1 \\
0 & 1 & 1 & 1 & 1 & 1 & 1 & 1 \\
1 & 0 & 0 & 0 & 1 & 0 & 0 & 1 \\
1 & 0 & 1 & 0 & 1 & 0 & 1 & 1 \\
1 & 1 & 0 & 1 & 0 & 0 & 0 & 1 \\ 
1 & 1 & 1 & 1 & 1 & 1 & 1 & 1 \\

\end{tabular}


10c.
$$[p \land (p \rightarrow q)] \rightarrow q$$

\begin{tabular}{c|c|c|c|c}
$p$ & $q$ & $p \rightarrow q$ & $p \land (p \rightarrow q)$ & $[p \land (p \rightarrow q)] \rightarrow q$ \\
\hline
0 & 0 & 1 & 0 & 1 \\
0 & 1 & 1 & 0 & 1 \\
1 & 0 & 0 & 0 & 1 \\
1 & 1 & 1 & 1 & 1 \\
\end{tabular}

10d.
$$[(p \land q) \land (p \rightarrow r) \land (q \rightarrow r)] \rightarrow r$$

\begin{tabular}{c|c|c|c|c|c|c|c}
$p$ &
$q$ &
$r$ &
$p \land q$ &
$p \rightarrow r$ &
$q \rightarrow r$ &
$(p \land q) \land (p \rightarrow r) \land (q \rightarrow r)$ &
$[(p \land q) \land (p \rightarrow r) \land (q \rightarrow r)] \rightarrow r$ \\
\hline
0 & 0 & 0 & 0 & 1 & 1 & 0 & 1\\
0 & 0 & 1 & 0 & 1 & 1 & 0 & 1\\
0 & 1 & 0 & 0 & 1 & 0 & 0 & 1\\
0 & 1 & 1 & 0 & 1 & 1 & 0 & 1\\
1 & 0 & 0 & 0 & 0 & 1 & 0 & 1\\
1 & 0 & 1 & 0 & 1 & 1 & 0 & 1\\
1 & 1 & 0 & 1 & 0 & 0 & 0 & 1\\
1 & 1 & 1 & 1 & 1 & 1 & 1 & 1\\
\end{tabular}

14
$$(\lnot p \land (p \rightarrow q)) \rightarrow \lnot q$$

\begin{tabular}{c|c|c|c|c|c}
$p$ &
$q$ &
$\lnot p$ &
$p \rightarrow q$ &
$\lnot p \land (p \rightarrow q)$ &
$(\lnot p \land (p \rightarrow q)) \rightarrow \lnot q$ \\
\hline
0 & 0 & 1 & 1 & 1 & 1 \\
0 & 1 & 1 & 1 & 1 & 1 \\
1 & 0 & 0 & 0 & 0 & 1 \\
1 & 1 & 0 & 1 & 0 & 1 \\
\end{tabular}

16
Is $p \leftrightarrow q \equiv (p \land q) \lor (\lnot p \land \lnot q)$?

\begin{tabular}{c|c|c|c|c|c}
$p$ &
$q$ &
$p \land q$ & 
$\lnot p \land \lnot q$ &
$(p \land q) \lor (\lnot p \land \lnot q)$ &
$p \leftrightarrow q$ \\
\hline
0 & 0 & 0 & 1 & 1 & 1 \\
0 & 1 & 0 & 0 & 0 & 0 \\
1 & 0 & 0 & 0 & 0 & 0 \\
1 & 1 & 1 & 0 & 1 & 1 \\
\end{tabular}

yes

18
Is $p \rightarrow q \equiv \lnot q \rightarrow p$?

\begin{tabular}{c|c|c|c}
$p$ &
$q$ &
$p \rightarrow q$ &
$\lnot q \rightarrow \lnot p$ \\
\hline
0 & 0 & 1 & 1 \\
0 & 1 & 1 & 1 \\
1 & 0 & 0 & 0 \\
1 & 1 & 1 & 1 \\
\end{tabular}
yes

20

\begin{tabular}{c|c|c|c|c}
$p$ &
$q$ &
$p \leftrightarrow q$ &
$q \oplus p$ &
$\lnot(q \oplus p)$ \\
\hline
0 & 0 & 1 & 1 & 1 \\
0 & 1 & 0 & 0 & 0 \\
1 & 0 & 0 & 0 & 0 \\
1 & 1 & 1 & 1 & 1 \\
\end{tabular}

62a. Yes, $p = T, q = F$

62b. Yes, $p = F, q = T, r = F$

62c. Yes, $p = T, q = T, r = F, s = T$

4a. 0

4b. 1

4c. 1

12a. True

12b. True

12c. False

12d. True

12e. Flase

12f. True

12g. False

14a. True

14b. True

14c. True

14d. False

20a. $P(-5) \lor P(-3) \lor \dots \lor P(5)$

20b. $P(-5) \land P(-3) \land \dots \land P(5)$

20c. $(x = 1) \lor (x \neq 1 \land \lnot P(x))$

20d. $(x \geq 0) \land (P(1) \lor P(3) \lor P(5))$

36a. x = 1

36b. x = 2

36c. x = 0

26a. False

26b. True

26c. False

26d. False

26e. True

26f. True

26g. True 

26h. False

26i. False

28a. True

28b. True

28c. True

28d. False

28e. True

28f. True

28g. True

28h. 
$$x + 2y = 2$$
$$x = 2 - 2y$$
$$2x + 4y = 5$$
$$2(2-2y) + 4y = 5$$
$$4 - 4y + 4y  = 5$$
$$0 = 5$$
False

28i.
$$x+y = 2$$
$$x = 2 - y$$

$$2(2-y) - y = 1$$
$$4 - y = 1$$
$$y = 3$$

False, $x=0$, $y=3$ does not work.

28j.
True

\end{document}
